sas_plus_plus_to_ω_imp_minus_minus

IMP--_To_SAS+/Correctness.thy
@@ -5,64 +5,11 @@ section "Correctness"
 theory Correctness imports Reduction SAS_Plus_Plus_Semantics
 begin 
 
-definition imp_minus_state_to_sas_plus :: "(com \<times> imp_state) \<Rightarrow> sas_state" where
-"imp_minus_state_to_sas_plus ci = ((\<lambda>x. Some (EV x)) \<circ>\<^sub>m (snd ci)
-  \<circ>\<^sub>m (\<lambda>x. (case x of VN v \<Rightarrow> Some v)))
-  (PC \<mapsto> PCV (fst ci))"
-
-definition sas_plus_state_to_imp_minus:: "sas_state \<Rightarrow> (com \<times> imp_state)" where
-"sas_plus_state_to_imp_minus ss = ((case (the (ss PC)) of (PCV c) \<Rightarrow> c), 
-  (\<lambda>x. (case x of EV y \<Rightarrow> Some y | _ \<Rightarrow> None)) \<circ>\<^sub>m ss \<circ>\<^sub>m (\<lambda>x. Some (VN x)))"
-
-definition sane_sas_plus_state:: "sas_state \<Rightarrow> bool" where
-"sane_sas_plus_state ss \<equiv> (\<exists>x. ss PC = Some (PCV x)) \<and> 
-  (\<forall>v. VN v \<in> dom ss \<longrightarrow> (\<exists>x. ss (VN v) = Some (EV x)))"
-
-lemma [simp]: "sas_plus_state_to_imp_minus (imp_minus_state_to_sas_plus (c, is)) = (c, is)" 
-proof -
-  have "(snd (sas_plus_state_to_imp_minus (imp_minus_state_to_sas_plus (c, is)))) x = is x" for x
-    by (auto simp: imp_minus_state_to_sas_plus_def sas_plus_state_to_imp_minus_def 
-        map_comp_def option.case_eq_if)
-  then show ?thesis
-    by (auto simp: imp_minus_state_to_sas_plus_def sas_plus_state_to_imp_minus_def)
-qed
-
-lemma [simp]: 
-  assumes "sane_sas_plus_state ss "
-  shows "imp_minus_state_to_sas_plus (sas_plus_state_to_imp_minus ss) = ss" 
-proof -
-  have "(imp_minus_state_to_sas_plus (sas_plus_state_to_imp_minus ss)) x = ss x" for x using assms
-    by (fastforce simp: imp_minus_state_to_sas_plus_def sas_plus_state_to_imp_minus_def 
-        sane_sas_plus_state_def option.case_eq_if map_comp_def split: variable.splits)
-  then show ?thesis by (auto simp: imp_minus_state_to_sas_plus_def sas_plus_state_to_imp_minus_def)
-qed
-
-lemma [simp]: "sas_plus_state_to_imp_minus 
-  ((imp_minus_state_to_sas_plus (c, is))(VN x \<mapsto> EV y, PC \<mapsto> PCV z)) 
-  = (z, (is(x \<mapsto> y)))"
-  by (auto simp: imp_minus_state_to_sas_plus_def sas_plus_state_to_imp_minus_def option.case_eq_if 
-      map_comp_def)
-
-lemma [simp]: "(imp_minus_state_to_sas_plus (c, s1) = imp_minus_state_to_sas_plus (c, s2))
-  \<longleftrightarrow> s1 = s2" 
-proof
-  assume a: "imp_minus_state_to_sas_plus (c, s1) = imp_minus_state_to_sas_plus (c, s2)"
-  have "\<forall>v. (s1 v = s2 v)"
-  proof (rule ccontr)
-    assume "\<not> (\<forall>v. s1 v = s2 v)"
-    then obtain v where "s1 v \<noteq> s2 v" by blast
-    then have "imp_minus_state_to_sas_plus (c, s1) (VN v) \<noteq> imp_minus_state_to_sas_plus (c, s2) (VN v)"
-      by (auto simp: imp_minus_state_to_sas_plus_def map_comp_def domD domIff split: option.splits)
-    then show "False" using a by simp
-  qed
-  then show "s1 = s2" by auto
-qed auto
-
 lemma sas_plus_state_to_imp_minus_of_effect: 
   assumes "op \<in> set (com_to_operators c1 (domain cA t))"
   shows "sas_plus_state_to_imp_minus (imp_minus_state_to_sas_plus (c, is) ++ map_of (effect_of op)) 
-  = (pc_to_com (effect_of op), is 
-  ++ ((\<lambda>x. (case x of EV y \<Rightarrow> Some y | _ \<Rightarrow> None)) \<circ>\<^sub>m (map_of (effect_of op)) \<circ>\<^sub>m (\<lambda>x. Some (VN x))))"
+  = (pc_to_com (effect_of op), 
+  snd (sas_plus_state_to_imp_minus (imp_minus_state_to_sas_plus (c, is) ++ map_of (effect_of op))))"
 proof -
   have "fst (sas_plus_state_to_imp_minus 
     (imp_minus_state_to_sas_plus (c, is) ++ map_of (effect_of op))) = pc_to_com (effect_of op)"
@@ -82,11 +29,6 @@ proof -
   ultimately show ?thesis using assms by (metis prod.collapse)
 qed
 
-lemma [simp]: "imp_minus_state_to_sas_plus (c1, is) = ss
-  \<Longrightarrow> v \<in> set (enumerate_variables c)
-  \<Longrightarrow> is v = Some (Num 0) \<longleftrightarrow> ss (VN v) = Some (EV (Num 0))"
-  by (auto simp: imp_minus_state_to_sas_plus_def option.case_eq_if map_comp_def split: if_splits)
-
 lemma [simp]: "(imp_minus_state_to_sas_plus (c1, is1))(PC \<mapsto> PCV c2) 
   = imp_minus_state_to_sas_plus (c2, is1)"
   by(auto simp: imp_minus_state_to_sas_plus_def option.case_eq_if)
@@ -105,6 +47,17 @@ lemma [simp]: "(imp_minus_state_to_sas_plus (c, s) (VN x) = Some y)
   \<longleftrightarrow> ((map_option EV (s x)) = Some y)"
   by (simp add: imp_minus_state_to_sas_plus_def map_comp_Some_iff)
 
+lemma [simp]: "op \<in> set (com_to_operators c (domain cA t)) 
+  \<Longrightarrow> (s ++ map_of (effect_of op)) (PC \<mapsto> PCV (pc_to_com (effect_of op))) = s ++ map_of (effect_of op)"
+  by (simp add: com_to_operators_variables_distinct fun_upd_idem)
+
+lemma imp_minus_state_to_sas_plus_add_effect: 
+  assumes "op \<in> set (com_to_operators c (domain cA t))"
+  shows "imp_minus_state_to_sas_plus (c1, is) ++ map_of (effect_of op) 
+      = imp_minus_state_to_sas_plus (pc_to_com (effect_of op), is) ++ map_of (effect_of op)"
+  using assms com_to_operators_variables_distinct 
+  by(auto simp: map_add_def imp_minus_state_to_sas_plus_def fun_eq_iff split: option.splits)
+  
 lemma imp_minus_state_to_sas_plus_of_effect: 
   assumes "op \<in> set (com_to_operators cB (domain cA t))"
   shows "((imp_minus_state_to_sas_plus (c1, s) ++ map_of (effect_of op))(PC \<mapsto> PCV c2) =
@@ -156,17 +109,9 @@ proof -
     imp_minus_state_to_sas_plus ((pc_to_com (effect_of op)), s')) 
     \<longleftrightarrow> ((s ++ ((\<lambda>x. (case x of EV y \<Rightarrow> Some y | _ \<Rightarrow> None)) 
     \<circ>\<^sub>m map_of (effect_of op) \<circ>\<^sub>m (\<lambda>x. Some (VN x)))) = s')" 
-    using assms imp_minus_state_to_sas_plus_of_effect by simp
-  ultimately show ?thesis using assms imp_minus_state_to_sas_plus_def map_upd_eqD1 by fastforce
-qed
-
-lemma [simp]: "(\<lambda>v. case v of VN v \<Rightarrow> f v | PC \<Rightarrow> Some x) =
-    (\<lambda>v. case v of VN v \<Rightarrow> f v | PC \<Rightarrow> y)(PC \<mapsto> x)"
-proof - 
-  have "(case v of VN v \<Rightarrow> f v | PC \<Rightarrow> Some x) 
-    = ((\<lambda>v. case v of VN v \<Rightarrow> f v | PC \<Rightarrow> y)(PC \<mapsto> x)) v" for v
-    by (cases v) auto
-  then show ?thesis by auto
+    using assms imp_minus_state_to_sas_plus_of_effect by blast
+  ultimately show ?thesis using assms imp_minus_state_to_sas_plus_def map_upd_eqD1 
+    by (metis domain_element.inject fst_conv)
 qed
 
 lemma updated_state_is_sane:
@@ -176,8 +121,10 @@ lemma updated_state_is_sane:
 proof -
   have "\<exists>x. (VN v, EV x) \<in> set (effect_of op) \<or> map_of (effect_of op) (VN v) = None" for v
     using assms variables_in_effect by simp
-  then show ?thesis using assms
-    by(auto simp: sane_sas_plus_state_def com_to_operators_variables_distinct map_add_Some_iff)
+  then show ?thesis using assms 
+    apply(auto simp: sane_sas_plus_state_def com_to_operators_variables_distinct 
+        map_add_Some_iff) 
+    using in_set_effect by blast
 qed
 
 lemma [simp]: "(\<lambda>a. if a = PC then Some (PCV c2) 
@@ -203,7 +150,6 @@ proof-
   then show ?thesis by auto
 qed
 
-
 lemma [simp]: "(\<lambda>a. if a = PC then Some (PCV c2) 
    else (imp_minus_state_to_sas_plus (c1, is1)(VN x \<mapsto> EV y)) a) 
     = imp_minus_state_to_sas_plus (c2, is1(x \<mapsto> y))"
@@ -228,18 +174,6 @@ proof -
   then show ?thesis 
     using assms by (auto simp: imp_minus_state_to_sas_plus_def sas_plus_state_to_imp_minus_def)
 qed
-
-lemma [simp]: 
-  "snd (sas_plus_state_to_imp_minus
-                (imp_minus_state_to_sas_plus (c, is)(VN x \<mapsto> y))) 
-    = is(x := (case y of EV y' \<Rightarrow> Some y' | _ \<Rightarrow> None))"
-  by (auto simp: imp_minus_state_to_sas_plus_def sas_plus_state_to_imp_minus_def 
-      domain_def Let_def map_comp_def option.case_eq_if)
-
-lemma [simp]: "(is(x := case y of EV y' \<Rightarrow> Some y' | _ \<Rightarrow> None) = is(x \<mapsto> z)) 
-  \<longleftrightarrow> (y = EV z)"
-  apply(cases y)
-  using fun_upd_eqD map_upd_eqD1 by fastforce+
 
 lemma [simp]: " s(x := case z of EV z' \<Rightarrow> Some z' | _ \<Rightarrow> None) = (\<lambda>a. if a = x then Some y else s a)
   \<longleftrightarrow> (z = EV y)"
@@ -292,17 +226,6 @@ lemma [simp]: "[PC \<mapsto> x] \<subseteq>\<^sub>m s \<longleftrightarrow> (s P
 lemma [simp]: "[PC \<mapsto> x] \<subseteq>\<^sub>m (imp_minus_state_to_sas_plus (c1, is)) 
   = (x = PCV c1)"
   by (auto simp: map_le_def imp_minus_state_to_sas_plus_def)
-
-lemma [simp]: "(imp_minus_state_to_sas_plus (c1, is)) PC = Some (PCV c1)" 
-  by (simp add: imp_minus_state_to_sas_plus_def)
-
-lemma [simp]: "(imp_minus_state_to_sas_plus (c, is) (VN x) = Some (EV y)) 
-  \<longleftrightarrow> (is x = Some y)"
-  by(auto simp: imp_minus_state_to_sas_plus_def map_comp_Some_iff)
-
-lemma [simp]: "imp_minus_state_to_sas_plus (c, is) (VN x) = Some y \<Longrightarrow>
-       (y \<noteq> EV (Num 0)) \<longleftrightarrow> (is x \<noteq> Some (Num 0))"
-  by(auto simp: imp_minus_state_to_sas_plus_def map_comp_Some_iff)
 
 lemma map_of_list_update: "distinct (map fst l) \<Longrightarrow> length l > 0 \<Longrightarrow> fst (l ! 0) = x  \<Longrightarrow> z \<noteq> x
   \<Longrightarrow> map_of (list_update l 0 (x, y)) z = map_of l z"
@@ -363,6 +286,7 @@ proof -
   then show ?thesis by auto
 qed
 
+
 lemma sas_plus_to_imp_minus_minus_single_step:
   "op \<in> set (com_to_operators c1 (domain c t))
   \<Longrightarrow> c1 \<in> set (enumerate_subprograms c) \<Longrightarrow> t > 0 
@@ -400,29 +324,20 @@ next
   then show ?case using Seq
   proof (elim disjE)
     assume "cA \<noteq> SKIP"
-    then obtain op' where op'_def: "op' \<in> set (com_to_operators cA (domain c t)) 
-      \<and> op = (let c1' = pc_to_com (effect_of op') in 
+    then obtain op' where op'_def: "op' \<in> set (com_to_operators cA (domain c t))"
+      "op = (let c1' = pc_to_com (effect_of op') in 
       \<lparr> precondition_of = list_update (precondition_of op') 0 (PC, PCV (cA ;; cB)),
         effect_of = list_update (effect_of op') 0 (PC, PCV (c1' ;; cB))\<rparr>)" using Seq by auto
     let ?c1' = "pc_to_com (effect_of op')"
     let ?ss1' = "(imp_minus_state_to_sas_plus ((cA ;; cB), is1))(PC \<mapsto> PCV cA)"
     let ?ss2' = "((imp_minus_state_to_sas_plus ((cA ;; cB), is1)) \<then>\<^sub>+ op)(PC \<mapsto> PCV ?c1')"
-    have "cA \<in> set (enumerate_subprograms (cA ;; cB))" using c_in_all_subprograms_c by auto
-    then have "cA \<in> set (enumerate_subprograms c)" 
-      using Seq enumerate_subprograms_transitive by blast
-    moreover have "imp_minus_state_to_sas_plus (cA, is1) = ?ss1'" by auto
-    moreover have "map_of (precondition_of op') = (map_of (precondition_of op))(PC \<mapsto> PCV cA)"
-      using op'_def Seq com_to_operators_variables_distinct by auto
-    moreover then have "is_operator_applicable_in ?ss1' op'" 
-      using Seq op'_def by (metis is_operator_applicable_in_def map_le_upd)
-    moreover have "map_of (effect_of op') = map_of (effect_of op)(PC \<mapsto> PCV (pc_to_com (effect_of op')))"
-      using op'_def Seq com_to_operators_variables_distinct by auto
-    moreover then have "?ss1' \<then>\<^sub>+ op' = ?ss2'" using Seq op'_def
-      using calculation(3) effect_in_updated by blast
-    (* TODO: simplify this proof (Seq(1)) *)
-    ultimately have "(cA, is1) \<rightarrow>\<^bsub>t * max_constant c\<^esub> sas_plus_state_to_imp_minus ?ss2'" 
-      using Seq op'_def by metis
-    then show ?thesis using Seq op'_def by auto
+    have "cA \<in> set (enumerate_subprograms c)" 
+      using \<open>cA;;cB \<in> set (enumerate_subprograms c)\<close> c_in_all_subprograms_c
+      by (force intro!: enumerate_subprograms_transitive[where ?c2.0 = "cA;; cB"])
+    then have "(cA, is1) \<rightarrow>\<^bsub>t * max_constant c\<^esub> sas_plus_state_to_imp_minus ?ss2'"
+      using \<open>0 < t\<close> op'_def Seq  imp_minus_state_to_sas_plus_add_effect[where ?c1.0="cA;; cB"]
+      imp_minus_state_to_sas_plus_add_effect[where ?c1.0="cA"] by auto
+    then show ?thesis apply(auto) using op'_def by auto
   qed auto
 qed auto
 
@@ -607,15 +522,63 @@ proof -
     using imp_minus_minus_to_sas_plus[OF assms(1)] assms c_in_all_subprograms_c by auto
   moreover then have "(?\<Psi>)\<^sub>G\<^sub>+ \<subseteq>\<^sub>m execute_serial_plan_sas_plus ?I' plan"
     and "dom ?I' = set (((?\<Psi>))\<^sub>\<V>\<^sub>+)"
+    and "(\<forall> v \<in> set ((?\<Psi>)\<^sub>\<V>\<^sub>+). the (?I' v) \<in> range_of' ?\<Psi> v)"
     and "((?\<Psi>)\<^sub>I\<^sub>+) \<subseteq>\<^sub>m ?I'"
-    using assms plan_def
-    apply(auto simp: imp_minus_minus_to_sas_plus_def Let_def sas_state_by_pc_and_vars_def 
-        imp_minus_state_to_sas_plus_def map_comp_def map_le_def split: option.splits variable.splits)
-    by auto
+    using assms plan_def c_in_all_subprograms_c
+    apply(auto simp: imp_minus_minus_to_sas_plus_def Let_def 
+        range_of'_def imp_minus_state_to_sas_plus_def map_comp_def map_le_def)
+        apply (auto split: option.splits variable.splits EVal.splits)
+    by (metis domIff option.distinct option.inject)
   ultimately have "is_serial_solution_for_problem ?\<Psi> plan" 
     using assms
     by(auto simp: is_serial_solution_for_problem_def Let_def list_all_def ListMem_iff)
   then show ?thesis using plan_def by blast
 qed
 
+lemma sas_plus_plus_to_\<omega>_imp_minus_minus:
+  assumes "is_serial_solution_for_problem (imp_minus_minus_to_sas_plus c I G t) plan"
+    "length plan < t"
+    "EV ` (ran I) \<subseteq> set (domain c t)"
+    "EV ` (ran G) \<subseteq> set (domain c t)"
+  shows "\<exists>is1 is2 t'. (I|` set (enumerate_variables c)) \<subseteq>\<^sub>m is1 
+    \<and> (G|` set (enumerate_variables c)) \<subseteq>\<^sub>m is2 \<and> t' \<le> length plan 
+    \<and> (c, is1) \<rightarrow>\<^bsub>t * max_constant c \<^esub>\<^bsup>t'\<^esup> (SKIP, is2)" 
+proof -
+  let ?\<Psi> = "imp_minus_minus_to_sas_plus c I G t"
+  obtain I' where I'_def: "((?\<Psi>)\<^sub>I\<^sub>+) \<subseteq>\<^sub>m I' \<and> dom I' = set ((?\<Psi>)\<^sub>\<V>\<^sub>+) 
+        \<and> (\<forall>v \<in> set ((?\<Psi>)\<^sub>\<V>\<^sub>+). the (I' v) \<in> range_of' ?\<Psi> v)
+        \<and> ((?\<Psi>)\<^sub>G\<^sub>+) \<subseteq>\<^sub>m execute_serial_plan_sas_plus I' plan" 
+    using assms by (auto simp: is_serial_solution_for_problem_def Let_def)
+  let ?ss2 = "execute_serial_plan_sas_plus I' plan"
+  let ?is1 = "snd (sas_plus_state_to_imp_minus I')"
+  let ?is2 = "snd (sas_plus_state_to_imp_minus ?ss2)"
+  have "\<forall>v\<in>set (enumerate_variables c). (\<exists>y \<in> set (domain c t). I' (VN v) = Some y)" using I'_def 
+    apply (auto simp: imp_minus_minus_to_sas_plus_def Let_def range_of'_def)
+    by (metis domIff image_insert insertI1 insertI2 mk_disjoint_insert option.collapse)
+  then have "sane_sas_plus_state I'" using I'_def assms
+    apply (auto simp: sane_sas_plus_state_def imp_minus_minus_to_sas_plus_def Let_def map_le_def 
+         range_of'_def domain_def)
+    by (metis domIff insertI1 option.collapse)
+  then obtain t' where t'_def: " t' \<le> length plan \<and> sas_plus_state_to_imp_minus I' 
+    \<rightarrow>\<^bsub>t * max_constant c \<^esub>\<^bsup>t'\<^esup> sas_plus_state_to_imp_minus ?ss2"
+    using sas_plus_to_imp_minus_minus assms(1) assms(2) I'_def 
+    by (auto simp: is_serial_solution_for_problem_def Let_def list_all_def ListMem_iff) blast
+  moreover have "fst (sas_plus_state_to_imp_minus I') = c"
+    and "fst (sas_plus_state_to_imp_minus ?ss2) = SKIP"
+    using assms I'_def apply(auto simp: imp_minus_minus_to_sas_plus_def Let_def 
+         sas_plus_state_to_imp_minus_def map_le_def imp_minus_state_to_sas_plus_def
+        sane_sas_plus_state_def)
+    by (metis (no_types, lifting) domain_element.inject domain_element.simps option.sel 
+        option.inject variable.simps)+
+  ultimately have "((c, ?is1) \<rightarrow>\<^bsub>t * max_constant c \<^esub>\<^bsup>t'\<^esup> (SKIP, ?is2))" 
+    using I'_def by (metis prod.collapse)
+  moreover have "(I|` set (enumerate_variables c)) \<subseteq>\<^sub>m ?is1"
+    "(G|` set (enumerate_variables c)) \<subseteq>\<^sub>m ?is2"
+    using assms(2) I'_def 
+    by (auto simp: imp_minus_minus_to_sas_plus_def imp_minus_state_to_sas_plus_map_le_then Let_def 
+        range_of'_def)
+  ultimately show ?thesis  using I'_def t'_def by blast
+qed
+    
+    
 end
