IMP--_To_SAS+/State_Translations.thy
@@ -1,0 +1,96 @@
+\<^marker>\<open>creator Florian Keßler\<close>
+
+section "State Translations"
+
+theory State_Translations imports SAS_Plus_Plus_Representation Omega_Small_StepT
+begin
+
+datatype domain_element = EV EVal | PCV com
+
+datatype variable = VN vname | PC
+
+type_synonym sas_state = "(variable, domain_element) State_Variable_Representation.state"
+type_synonym imp_state = EState
+
+definition imp_minus_state_to_sas_plus :: "(com \<times> imp_state) \<Rightarrow> sas_state" where
+"imp_minus_state_to_sas_plus ci = ((\<lambda>x. Some (EV x)) \<circ>\<^sub>m (snd ci)
+  \<circ>\<^sub>m (\<lambda>x. (case x of VN v \<Rightarrow> Some v)))
+  (PC \<mapsto> PCV (fst ci))"
+
+definition sas_plus_state_to_imp_minus:: "sas_state \<Rightarrow> (com \<times> imp_state)" where
+"sas_plus_state_to_imp_minus ss = ((case (the (ss PC)) of (PCV c) \<Rightarrow> c), 
+  (\<lambda>x. (case x of EV y \<Rightarrow> Some y | _ \<Rightarrow> None)) \<circ>\<^sub>m ss \<circ>\<^sub>m (\<lambda>x. Some (VN x)))"
+
+definition sane_sas_plus_state:: "sas_state \<Rightarrow> bool" where
+"sane_sas_plus_state ss \<equiv> (\<exists>x. ss PC = Some (PCV x)) \<and> 
+  (\<forall>v. VN v \<in> dom ss \<longrightarrow> (\<exists>x. ss (VN v) = Some (EV x)))"
+
+lemma [simp]: "sas_plus_state_to_imp_minus (imp_minus_state_to_sas_plus (c, is)) = (c, is)" 
+proof -
+  have "(snd (sas_plus_state_to_imp_minus (imp_minus_state_to_sas_plus (c, is)))) x = is x" for x
+    by (auto simp: imp_minus_state_to_sas_plus_def sas_plus_state_to_imp_minus_def 
+        map_comp_def option.case_eq_if)
+  then show ?thesis
+    by (auto simp: imp_minus_state_to_sas_plus_def sas_plus_state_to_imp_minus_def)
+qed
+
+lemma [simp]: 
+  assumes "sane_sas_plus_state ss "
+  shows "imp_minus_state_to_sas_plus (sas_plus_state_to_imp_minus ss) = ss" 
+proof -
+  have "(imp_minus_state_to_sas_plus (sas_plus_state_to_imp_minus ss)) x = ss x" for x using assms
+    by (fastforce simp: imp_minus_state_to_sas_plus_def sas_plus_state_to_imp_minus_def 
+        sane_sas_plus_state_def option.case_eq_if map_comp_def split: variable.splits)
+  then show ?thesis by (auto simp: imp_minus_state_to_sas_plus_def sas_plus_state_to_imp_minus_def)
+qed
+
+lemma [simp]: "sas_plus_state_to_imp_minus 
+  ((imp_minus_state_to_sas_plus (c, is))(VN x \<mapsto> EV y, PC \<mapsto> PCV z)) 
+  = (z, (is(x \<mapsto> y)))"
+  by (auto simp: imp_minus_state_to_sas_plus_def sas_plus_state_to_imp_minus_def option.case_eq_if 
+      map_comp_def)
+
+lemma [simp]: "(imp_minus_state_to_sas_plus (c, s1) = imp_minus_state_to_sas_plus (c, s2))
+  \<longleftrightarrow> s1 = s2" 
+proof
+  assume a: "imp_minus_state_to_sas_plus (c, s1) = imp_minus_state_to_sas_plus (c, s2)"
+  have "\<forall>v. (s1 v = s2 v)"
+  proof (rule ccontr)
+    assume "\<not> (\<forall>v. s1 v = s2 v)"
+    then obtain v where "s1 v \<noteq> s2 v" by blast
+    then have "imp_minus_state_to_sas_plus (c, s1) (VN v) \<noteq> imp_minus_state_to_sas_plus (c, s2) (VN v)"
+      by (auto simp: imp_minus_state_to_sas_plus_def map_comp_def domD domIff split: option.splits)
+    then show "False" using a by simp
+  qed
+  then show "s1 = s2" by auto
+qed auto
+
+lemma [simp]: 
+  "snd (sas_plus_state_to_imp_minus
+                (imp_minus_state_to_sas_plus (c, is)(VN x \<mapsto> y))) 
+    = is(x := (case y of EV y' \<Rightarrow> Some y' | _ \<Rightarrow> None))"
+  by (auto simp: imp_minus_state_to_sas_plus_def sas_plus_state_to_imp_minus_def 
+       Let_def map_comp_def option.case_eq_if)
+
+lemma [simp]: "(imp_minus_state_to_sas_plus (c1, is)) PC = Some (PCV c1)" 
+  by (simp add: imp_minus_state_to_sas_plus_def)
+
+lemma [simp]: "(imp_minus_state_to_sas_plus (c, is) (VN x) = Some (EV y)) 
+  \<longleftrightarrow> (is x = Some y)"
+  by(auto simp: imp_minus_state_to_sas_plus_def map_comp_Some_iff)
+
+lemma [simp]: "imp_minus_state_to_sas_plus (c, is) (VN x) = Some y \<Longrightarrow>
+       (y \<noteq> EV (Num 0)) \<longleftrightarrow> (is x \<noteq> Some (Num 0))"
+  by(auto simp: imp_minus_state_to_sas_plus_def map_comp_Some_iff)
+
+lemma imp_minus_state_to_sas_plus_map_le_then: "imp_minus_state_to_sas_plus (c, I) \<subseteq>\<^sub>m I' 
+  \<Longrightarrow> I \<subseteq>\<^sub>m snd (sas_plus_state_to_imp_minus I')"
+  apply(auto simp: imp_minus_state_to_sas_plus_def sas_plus_state_to_imp_minus_def)
+   apply(simp add: map_le_def map_comp_def)
+   apply(auto split: option.splits domain_element.splits)
+     apply (metis domIff option.distinct option.simps variable.simps)
+   apply (metis domI domain_element.inject option.inject option.simps variable.distinct variable.simps)
+  by (metis (mono_tags, lifting) domI domain_element.distinct option.inject option.simps 
+      variable.distinct variable.simps)
+
+end
